coq/Completeness.v
@@ -1449,6 +1449,143 @@ Lemma completeness_single_step_shift : forall c cid v op w e1 e2 c' s,
   (exists s', sym_step s s' /\ over_approx s' c').
 Proof.
   intros c cid v op w e1 e2 c' s Hop Hcmd Hiss Hnp Hs Hws Hoa.
+  destruct c as [c_ic c_c c_cs c_pbid c_ls c_stk c_gs c_mdl].
+  destruct s as [s_ic s_c s_cs s_pbid s_ls s_stk s_gs s_syms s_pc s_mdl].
+  inversion Hs; subst.
+  inversion Hoa; subst.
+  inversion H; subst;
+  try discriminate Hcmd.
+  inversion Hoa; subst.
+  destruct H1 as [m H1].
+  inversion H1; subst.
+  inversion Hcmd; subst.
+  inversion Hnp; subst.
+  inversion Hiss; subst.
+  inversion H7; subst.
+  { inversion Hop; subst; inversion H4; subst; inversion H15. }
+  {
+    simpl in H11.
+    destruct
+      (eval_exp c_ls c_gs (Some (TYPE_I w)) e1) as [dv1 | ] eqn:E1,
+      (eval_exp c_ls c_gs (Some (TYPE_I w)) e2) as [dv2 | ] eqn:E2;
+    try discriminate H11.
+    destruct dv1 as [di1 | | ] , dv2 as [di2 | | ];
+    try (
+      unfold eval_ibinop in H11;
+      destruct di1; discriminate H11
+    );
+    try (
+      unfold eval_ibinop in H11;
+      destruct di2; discriminate H11
+    );
+    try (
+      unfold eval_ibinop in H11;
+      discriminate H11
+    );
+    try (
+      apply has_no_poison_eval_exp in E1; try assumption;
+      destruct E1; reflexivity
+    );
+    try (
+      apply has_no_poison_eval_exp in E2; try assumption;
+      destruct E2; reflexivity
+    ).
+    unfold eval_ibinop in H11.
+    destruct di1 as [n1 | n1 | n1 | n1 | n1], di2 as [n2 | n2 | n2 | n2 | n2];
+    try (discriminate H11).
+    {
+      assert(L1 :
+        over_approx_via_model
+          (eval_exp c_ls c_gs (Some (TYPE_I w)) e1)
+          (sym_eval_exp s_ls s_gs (Some (TYPE_I w)) e1)
+          m
+      ).
+      { apply eval_exp_correspondence; assumption. }
+      assert(L2 :
+        over_approx_via_model
+          (eval_exp c_ls c_gs (Some (TYPE_I w)) e2)
+          (sym_eval_exp s_ls s_gs (Some (TYPE_I w)) e2)
+          m
+      ).
+      { apply eval_exp_correspondence; assumption. }
+      rewrite E1 in L1.
+      rewrite E2 in L2.
+      inversion L1; subst.
+      inversion L2; subst.
+      rename sort into sort1, ast into ast1, sort0 into sort2, ast0 into ast2.
+      assert(Lsort1 : sort1 = Sort_BV1).
+      { eapply infer_sort. eassumption. }
+      assert(Lsort2 : sort2 = Sort_BV1).
+      { eapply infer_sort. eassumption. }
+      subst.
+      exists (mk_sym_state
+        (next_inst_counter c_ic c)
+        c
+        cs
+        c_pbid
+        (v !-> Some (Expr Sort_BV1 (AST_BinOp Sort_BV1 (ibinop_to_smt_binop op) ast1 ast2)); s_ls)
+        s_stk
+        s_gs
+        s_syms
+        s_pc
+        c_mdl
+      ).
+      split.
+      {
+        apply Sym_Step_OP.
+        simpl.
+        rewrite <- H4.
+        rewrite <- H5.
+        reflexivity.
+      }
+      {
+        apply OA_State.
+        exists m.
+        apply OAV_State; try assumption.
+        apply store_update_correspondence; try assumption.
+        destruct op; inversion Hop; subst.
+        {
+          rewrite <- H11.
+          simpl.
+          destruct (Int1.unsigned n2 >=? 1)%Z eqn:En2.
+          {
+            simpl in H11.
+            rewrite En2 in H11.
+            inversion H11; subst.
+            inversion H0; subst.
+            inversion H20; subst.
+            specialize (H3 v).
+            rewrite update_map_eq in H3.
+            destruct H3.
+            reflexivity.
+          }
+          {
+            eapply OA_Some.
+            { reflexivity. }
+            {
+              simpl.
+              simpl in H11.
+              rewrite En2 in H11.
+              inversion H11; subst.
+              assert(Ln2 : n2 = Int1.repr 0).
+              { apply int1_lt_one. assumption. }
+              inversion H12; subst.
+              rewrite H10.
+              rewrite Int1.shl_zero.
+              inversion H9; subst.
+              reflexivity.
+            }
+          }
+        }
+        { admit. }
+        { admit. }
+      }
+    }
+    { admit. }
+    { admit. }
+    { admit. }
+    { admit. }
+  }
 Admitted.
 
 (* TODO: (has_no_poison c) can be inferred from (over_approx s c)? *)
@@ -1549,121 +1686,10 @@ Proof.
       }
       (* Shl *)
       {
-        simpl in H10.
-        destruct
-          (eval_exp c_ls c_gs (Some (TYPE_I w)) e1) as [dv1 | ] eqn:E1,
-          (eval_exp c_ls c_gs (Some (TYPE_I w)) e2) as [dv2 | ] eqn:E2;
-        try discriminate H10.
-        destruct dv1 as [di1 | | ] , dv2 as [di2 | | ];
-        try (
-          unfold eval_ibinop in H10;
-          destruct di1; discriminate H10
-        );
-        try (
-          unfold eval_ibinop in H10;
-          destruct di2; discriminate H10
-        );
-        try (
-          unfold eval_ibinop in H10;
-          discriminate H10
-        );
-        try (
-          apply has_no_poison_eval_exp in E1; try assumption;
-          destruct E1; reflexivity
-        );
-        try (
-          apply has_no_poison_eval_exp in E2; try assumption;
-          destruct E2; reflexivity
-        ).
-        unfold eval_ibinop in H10.
-        destruct di1 as [n1 | n1 | n1 | n1 | n1], di2 as [n2 | n2 | n2 | n2 | n2];
-        try (discriminate H10).
-        {
-          simpl in H10.
-          destruct (Int1.unsigned n2 >=? 1)%Z eqn:En2.
-          {
-            inversion H10; subst.
-            inversion H0; subst.
-            inversion H11; subst.
-            specialize (H2 v).
-            rewrite update_map_eq in H2.
-            destruct H2.
-            reflexivity.
-          }
-          {
-            assert(L1 :
-              over_approx_via_model
-                (eval_exp c_ls c_gs (Some (TYPE_I w)) e1)
-                (sym_eval_exp s_ls s_gs (Some (TYPE_I w)) e1)
-                m
-            ).
-            { apply eval_exp_correspondence; assumption. }
-            assert(L2 :
-              over_approx_via_model
-                (eval_exp c_ls c_gs (Some (TYPE_I w)) e2)
-                (sym_eval_exp s_ls s_gs (Some (TYPE_I w)) e2)
-                m
-            ).
-            { apply eval_exp_correspondence; assumption. }
-            rewrite E1 in L1.
-            rewrite E2 in L2.
-            inversion L1; subst.
-            inversion L2; subst.
-            rename sort into sort1, ast into ast1, sort0 into sort2, ast0 into ast2.
-            assert(Lsort1 : sort1 = Sort_BV1).
-            { eapply infer_sort. eassumption. }
-            assert(Lsort2 : sort2 = Sort_BV1).
-            { eapply infer_sort. eassumption. }
-            subst.
-            exists (mk_sym_state
-              (next_inst_counter c_ic c)
-              c
-              cs
-              c_pbid
-              (v !-> Some (Expr Sort_BV1 (AST_BinOp Sort_BV1 SMT_Shl ast1 ast2)); s_ls)
-              s_stk
-              s_gs
-              s_syms
-              s_pc
-              c_mdl
-            ).
-            split.
-            {
-              apply Sym_Step_OP.
-              simpl.
-              rewrite <- H3.
-              rewrite <- H4.
-              reflexivity.
-            }
-            {
-              apply OA_State.
-              exists m.
-              apply OAV_State; try assumption.
-              apply store_update_correspondence.
-              {
-                rewrite <- H10.
-                eapply OA_Some.
-                { reflexivity. }
-                {
-                  simpl.
-                  inversion H11; subst.
-                  assert(Ln2 : n2 = Int1.repr 0).
-                  { apply int1_lt_one. assumption. }
-                  inversion H17; subst.
-                  rewrite H14.
-                  rewrite Int1.shl_zero.
-                  reflexivity.
-                }
-              }
-              { assumption. }
-            }
-          }
-        }
-        (* TODO: should be similar *)
-        { admit. }
-        { admit. }
-        { admit. }
-        { admit. }
+        eapply completeness_single_step_shift
+          with (cid := cid) (v := v) (w := w) (e1 := e1) (e2 := e2); try eassumption.
+        { apply Is_Unsafe_Shift_Shl. }
+        { reflexivity. }
       }
       (* LShr *)
       {
